some code for doing syntax diff

SyntaxDiff/Program.cs
@@ -1,0 +1,110 @@
+﻿using Microsoft.VisualStudio.Text;
+using Microsoft.VisualStudio.Text.Differencing;
+using Microsoft.VisualStudio.Utilities;
+using SourceAnalyzer;
+using System;
+using System.Collections.Generic;
+using System.ComponentModel.Composition;
+using System.ComponentModel.Composition.Hosting;
+using System.Diagnostics;
+using System.IO;
+using System.Linq;
+using System.Reflection;
+using System.Text;
+using System.Threading.Tasks;
+
+
+
+namespace SyntaxDiff
+{
+    /// <summary>
+    /// Generate the syntax diff information
+    /// </summary>
+    class Program
+    {
+        static void Main(string[] args)
+        {
+            var diffInfo = new DiffInfo();
+            Debug.Assert(args.Count() >= 2);
+            var diffOut = diffInfo.PerformDiffString(args[0], args[1]);
+        }
+
+    }
+    class DiffInfo
+    {
+        //MEF compoennts dir
+        public const string componentsDir = @"D:\vmv-analysis\VMV\";
+
+        [Import]
+        IHierarchicalStringDifferenceService differenceService = null;
+        public DiffInfo() { LoadMEFComponents(); }
+        public void LoadMEFComponents()
+        {
+            string[] ComponentDllFilters = new string[] { /*"CodeFlow*.exe", "Microsoft.CodeFlow.*.dll", */ "Delta.dll", "Microsoft.VisualStudio*.dll" };
+            /* this is lame and needs to be set for the machine that it is running on
+             * There is probably a way to autodetect this, but I don't know it */
+
+            //string componentsDir = "./";// ConfigurationManager.AppSettings["ComponentsDIR"];
+            AggregateCatalog catalog = new AggregateCatalog();
+            foreach (string filter in ComponentDllFilters)
+            {
+                catalog.Catalogs.Add(new DirectoryCatalog(componentsDir, filter));
+            }
+
+            try
+            {
+                CompositionBatch batch = new CompositionBatch();
+                batch.AddPart(this);
+
+                CompositionContainer container = new CompositionContainer(catalog, isThreadSafe: true);
+                container.Compose(batch);
+            }
+            catch (ReflectionTypeLoadException ex)
+            {
+                foreach (Exception loaderException in ex.LoaderExceptions)
+                {
+                    Console.WriteLine(loaderException.ToString());
+                }
+                throw;
+            }
+        }
+        public HashSet<Tuple<int, int>> PerformDiffFiles(string file1, string file2)
+        {
+            HashSet<Tuple<int, int>> diffRanges = new HashSet<Tuple<int, int>>();
+            StringDifferenceOptions sdo = new StringDifferenceOptions()
+            {
+                DifferenceType = StringDifferenceTypes.Line | StringDifferenceTypes.Word,
+                IgnoreTrimWhiteSpace = false
+            };
+
+            var origContent = (new StreamReader(file1)).ReadToEnd();
+            var modifiedContent = (new StreamReader(file2)).ReadToEnd();
+            var diffs = differenceService.DiffStrings(origContent, modifiedContent, sdo);
+            var diffList = new List<CCDifference>();
+            foreach (var d in diffs)
+            {
+                diffList.Add(new CCDifference(d.Left, d.Right, d.Before, d.After));
+                diffRanges.Add(Tuple.Create<int, int>(d.Left.Start, d.Left.End));
+            }
+            return diffRanges;
+        }
+        public HashSet<Tuple<int, int>> PerformDiffString(string origContent, string modifiedContent)
+        {
+            HashSet<Tuple<int, int>> diffRanges = new HashSet<Tuple<int, int>>();
+            StringDifferenceOptions sdo = new StringDifferenceOptions()
+            {
+                DifferenceType = StringDifferenceTypes.Line | StringDifferenceTypes.Word,
+                IgnoreTrimWhiteSpace = false
+            };
+
+            var diffs = differenceService.DiffStrings(origContent, modifiedContent, sdo);
+            var diffList = new List<CCDifference>();
+            foreach (var d in diffs)
+            {
+                diffList.Add(new CCDifference(d.Left, d.Right, d.Before, d.After));
+                diffRanges.Add(Tuple.Create<int, int>(d.Left.Start, d.Left.End));
+            }
+            return diffRanges;
+        }
+    }
+}
